adding axioms (#1)
* adding axioms

* rm checks and stuff

src/Semantics/Proof.v
@@ -13,19 +13,27 @@ Require Import IFOL.Syntax.Proof.
 Require Import IFOL.Semantics.Signature.
 Require Import IFOL.Semantics.Term.
 Require Import IFOL.Semantics.Formula.
+Require Import IFOL.Semantics.Theory.
 
 Definition seq_dom {S} {sg : sig S} {env}
   (eval_S : sort_dom S) (eval_sig : sig_dom eval_S sg) (args : env_dom eval_S env)
   (seq : BList (Formula sg) env) : Type :=
   BVec (eval_Formula eval_S sg eval_sig) args seq.
 
-Fixpoint eval_Proof {S} eval_S {sg : sig S} {env}
+Fixpoint eval_Proof {S} eval_S {sg : sig S} {env} {th}
   {seq : BList (Formula sg) env} eval_sig args {phi}
+  (eval_th : theory_dom eval_S sg eval_sig th)
   (eval_seq : seq_dom eval_S eval_sig args seq)
-  (pf : Proof seq phi) :
+  (pf : Proof th seq phi) :
   eval_Formula eval_S sg eval_sig env args phi.
 Proof.
   destruct pf eqn:?.
+  - unfold theory_dom in eval_th.
+    pose (eval_th i).
+    apply eval_Formula_suff_weaken.
+    destruct (RHVec.rhv_suff (sw_nil env) args).
+    simpl.
+    exact e.
   - unfold seq_dom in eval_seq.
     pose proof (bv_proj eval_seq i).
     unfold proj_with_weakenings.
@@ -34,43 +42,43 @@ Proof.
     apply eval_Formula_suff_weaken.
     exact H.
   - destruct (
-      eval_Proof S eval_S sg env seq eval_sig args _ eval_seq p).
+      eval_Proof S eval_S sg env th seq eval_sig args _ eval_th eval_seq p).
   - exact I.
   - left.
-    exact (eval_Proof S eval_S sg env seq eval_sig args _ eval_seq p).
+    exact (eval_Proof S eval_S sg env th seq eval_sig args _ eval_th eval_seq p).
   - right.
-    exact (eval_Proof S eval_S sg env seq eval_sig args _ eval_seq p).
+    exact (eval_Proof S eval_S sg env th seq eval_sig args _ eval_th eval_seq p).
   - simpl in p1.
     destruct (
-      eval_Proof S eval_S sg env seq eval_sig args _ eval_seq p1).
+      eval_Proof S eval_S sg env th seq eval_sig args _ eval_th eval_seq p1).
     + pose (eval_seq' :=
       bvcons _ H eval_seq).
-      exact (eval_Proof S eval_S sg env _ eval_sig args _ eval_seq' p2).
+      exact (eval_Proof S eval_S sg env th _ eval_sig args _ eval_th eval_seq' p2).
     + pose (eval_seq' :=
       bvcons _ H eval_seq).
-      exact (eval_Proof S eval_S sg env _ eval_sig args _ eval_seq' p3).
+      exact (eval_Proof S eval_S sg env th _ eval_sig args _ eval_th eval_seq' p3).
   - exact (conj
-      (eval_Proof S eval_S sg env seq eval_sig args _ eval_seq p1)
-      (eval_Proof S eval_S sg env seq eval_sig args _ eval_seq p2)
+      (eval_Proof S eval_S sg env th seq eval_sig args _ eval_th eval_seq p1)
+      (eval_Proof S eval_S sg env th seq eval_sig args _ eval_th eval_seq p2)
     ).
   - exact (proj1
-      (eval_Proof S eval_S sg env seq eval_sig args _ eval_seq p)
+      (eval_Proof S eval_S sg env th seq eval_sig args _ eval_th eval_seq p)
     ).
   - exact (proj2
-      (eval_Proof S eval_S sg env seq eval_sig args _ eval_seq p)
+      (eval_Proof S eval_S sg env th seq eval_sig args _ eval_th eval_seq p)
     ).
   - intro q.
     pose (eval_seq' :=
       bvcons _ q eval_seq).
-    exact (eval_Proof S eval_S sg env _ eval_sig args _ eval_seq' p).
+    exact (eval_Proof S eval_S sg env th _ eval_sig args _ eval_th eval_seq' p).
   - simpl.
-    apply (eval_Proof S eval_S sg env _ eval_sig args _ eval_seq p1).
-    exact (eval_Proof S eval_S sg env _ eval_sig args _ eval_seq p2).
+    apply (eval_Proof S eval_S sg env th _ eval_sig args _ eval_th eval_seq p1).
+    exact (eval_Proof S eval_S sg env th _ eval_sig args _ eval_th eval_seq p2).
   - simpl.
     intro.
-    exact (eval_Proof S eval_S sg (cons s env) _ eval_sig (x, args) _
+    exact (eval_Proof S eval_S sg (cons s env) th _ eval_sig (x, args) _ eval_th
       (bv_bump _ _ eval_seq) p).
-  - epose (eval_Proof S eval_S sg _ _ eval_sig args _ eval_seq p).
+  - epose (eval_Proof S eval_S sg _ th _ eval_sig args _ eval_th eval_seq p).
     simpl in e.
     epose (eval_Term eval_S (func_dom _ _ eval_sig) args t).
     pose (e e0).
@@ -78,17 +86,17 @@ Proof.
     rewrite eval_Formula_subst.
     exact e1.
   - exists (eval_Term eval_S (func_dom _ _ eval_sig) args t).
-    epose (eval_Proof S eval_S sg _ _ eval_sig args _ eval_seq p).
+    epose (eval_Proof S eval_S sg _ th _ eval_sig args _ eval_th eval_seq p).
     rewrite eval_Formula_subst in e.
     exact e.
-  - destruct (eval_Proof S eval_S sg _ _ eval_sig args _ eval_seq p1)
+  - destruct (eval_Proof S eval_S sg _ th _ eval_sig args _ eval_th eval_seq p1)
       as [x pf_x].
-    epose proof (eval_Proof S eval_S sg (cons s env) (bcons phi (bump s seq)) eval_sig (x, args) _
-      (pf_x, tt, eval_seq) p2).
+    epose proof (eval_Proof S eval_S sg (cons s env) th (bcons phi (bump s seq)) eval_sig (x, args) _
+      eval_th (pf_x, tt, eval_seq) p2).
     eapply eval_Formula_weaken; exact H.
   - reflexivity.
-  - pose (eval_Proof S eval_S sg _ _ eval_sig args _ eval_seq p1).
-    pose (eval_Proof S eval_S sg _ _ eval_sig args _ eval_seq p2).
+  - pose (eval_Proof S eval_S sg _ th _ eval_sig args _ eval_th eval_seq p1).
+    pose (eval_Proof S eval_S sg _ th _ eval_sig args _ eval_th eval_seq p2).
     simpl in e0.
     now rewrite eval_Formula_subterm_subst in e.
 Defined.
