src/Syntax/Proof.v
@@ -4,14 +4,7 @@ Require Import IFOL.Util.Witness.
 Require Import IFOL.Syntax.Signature.
 Require Import IFOL.Syntax.Term.
 Require Import IFOL.Syntax.Formula.
-
-Lemma foo {S} {sg : sig S} :
-  forall x env, Formula sg env -> Formula sg (x :: env).
-  intros.
-  eapply Formula_weaken.
-  - exact pwhd.
-  - exact X.
-Defined.
+Require Import IFOL.Syntax.Theory.
 
 Fixpoint suff_weaken {S} {sg : sig S} {env suff}
   (suff_wit : suffix_wit suff env) : Formula sg suff -> Formula sg env.
@@ -32,63 +25,65 @@ Proof.
   exact (data _ b).
 Defined.
 
-Inductive Proof {S} {sg : sig S} : forall {env},
+Inductive Proof {S} {sg : sig S} (th : Theory sg) : forall {env},
   BList (Formula sg) env -> Formula sg env -> Type :=
+  | Ax (i : carrier sg th) {env} {seq : BList (Formula sg) env}
+      : Proof th seq (suff_weaken (sw_nil _) (formula sg th i))
   | Assumption {env} {seq : BList (Formula sg) env}
       (i : bindex seq)
-      : Proof seq (proj_with_weakenings seq i)
+      : Proof th seq (proj_with_weakenings seq i)
   | Bot_elim {env} {seq : BList (Formula sg) env} phi :
-      Proof seq (NullProp _ Bot) -> Proof seq phi
+      Proof th seq (NullProp _ Bot) -> Proof th seq phi
   | Top_intro {env} {seq : BList (Formula sg) env} :
-      Proof seq (NullProp _ Top)
+      Proof th seq (NullProp _ Top)
   | Sum_intro_l {env} {seq : BList (Formula sg) env} phi psi :
-      Proof seq phi -> Proof seq (BinProp _ Sum phi psi)
+      Proof th seq phi -> Proof th seq (BinProp _ Sum phi psi)
   | Sum_intro_r {env} {seq : BList (Formula sg) env} phi psi :
-      Proof seq psi -> Proof seq (BinProp _ Sum phi psi)
+      Proof th seq psi -> Proof th seq (BinProp _ Sum phi psi)
   | Sum_elim {env} {seq : BList (Formula sg) env} phi psi rho :
-      Proof seq (BinProp _ Sum phi psi) ->
-      Proof (bcons phi seq) rho -> Proof (bcons psi seq) rho ->
-      Proof seq rho
+      Proof th seq (BinProp _ Sum phi psi) ->
+      Proof th (bcons phi seq) rho -> Proof th (bcons psi seq) rho ->
+      Proof th seq rho
   | Prod_intro {env} {seq : BList (Formula sg) env} phi psi :
-      Proof seq phi -> Proof seq psi ->
-      Proof seq (BinProp _ Prod phi psi)
+      Proof th seq phi -> Proof th seq psi ->
+      Proof th seq (BinProp _ Prod phi psi)
   | Prod_elim_l {env} {seq : BList (Formula sg) env} phi psi :
-      Proof seq (BinProp _ Prod phi psi) ->
-      Proof seq phi
+      Proof th seq (BinProp _ Prod phi psi) ->
+      Proof th seq phi
   | Prod_elim_r {env} {seq : BList (Formula sg) env} phi psi :
-      Proof seq (BinProp _ Prod phi psi) ->
-      Proof seq psi
+      Proof th seq (BinProp _ Prod phi psi) ->
+      Proof th seq psi
   | Exp_intro {env} {seq : BList (Formula sg) env} phi psi :
-      Proof (bcons phi seq) psi ->
-      Proof seq (BinProp _ Exp phi psi)
+      Proof th (bcons phi seq) psi ->
+      Proof th seq (BinProp _ Exp phi psi)
   | Exp_elim {env} {seq : BList (Formula sg) env} phi psi :
-      Proof seq (BinProp _ Exp phi psi) ->
-      Proof seq phi ->
-      Proof seq psi
+      Proof th seq (BinProp _ Exp phi psi) ->
+      Proof th seq phi ->
+      Proof th seq psi
   | Pi_intro {env} {seq} s
       (phi : Formula sg (s :: env)) :
-      Proof (bump s seq) phi -> Proof seq (QuantifierProp _ _ Pi phi)
+      Proof th (bump s seq) phi -> Proof th seq (QuantifierProp _ _ Pi phi)
   | Pi_elim {env} {seq} s
       (phi : Formula sg (s :: env)) :
-      Proof seq (QuantifierProp _ _ Pi phi) ->
+      Proof th seq (QuantifierProp _ _ Pi phi) ->
       forall (t : Term (func sg) env s),
-      Proof seq (Formula_subst pwhd t phi)
+      Proof th seq (Formula_subst pwhd t phi)
   | Sigma_intro {env} {seq} s
       (phi : Formula sg (s :: env))
       (t : Term (func sg) env s) :
-      Proof seq (Formula_subst pwhd t phi) ->
-      Proof seq (QuantifierProp _ _ Sigma phi)
+      Proof th seq (Formula_subst pwhd t phi) ->
+      Proof th seq (QuantifierProp _ _ Sigma phi)
   | Sigma_elim {env} {seq} s
       (phi : Formula sg (s :: env)) psi :
-      Proof seq (QuantifierProp _ _ Sigma phi) ->
-      Proof (bcons phi (bump s seq)) (Formula_weaken pwhd psi) ->
-      Proof seq psi
+      Proof th seq (QuantifierProp _ _ Sigma phi) ->
+      Proof th (bcons phi (bump s seq)) (Formula_weaken pwhd psi) ->
+      Proof th seq psi
   | Eq_intro {env} {seq} {s}
       (t : Term (func sg) env s) :
-      Proof seq (EqualityProp _ _ _ t t)
+      Proof th seq (EqualityProp _ _ _ t t)
   | Eq_elim {env} {seq} {s} phi
       (t u : Term (func sg) env s)
       (fw : Formula_subterm_witness t phi) :
-      Proof seq (Formula_subterm_subst phi fw u) ->
-      Proof seq (EqualityProp _ _ _ t u) ->
-      Proof seq phi.
+      Proof th seq (Formula_subterm_subst phi fw u) ->
+      Proof th seq (EqualityProp _ _ _ t u) ->
+      Proof th seq phi.
