src/Syntax/Theory.v
@@ -1,0 +1,7 @@
+Require Import IFOL.Syntax.Signature.
+Require Import IFOL.Syntax.Formula.
+
+Record Theory {S} (sg : sig S) : Type := {
+  carrier : Type;
+  formula : carrier -> Formula sg nil
+  }.
